progress on proving main thm and lemmas

vt/PikeVM_VT.v
@@ -36,6 +36,7 @@ to the next position where the prefix matches.
 
 From Stdlib Require Import List Lia.
 Import ListNotations.
+From Stdlib Require Import Program.Equality.
 
 From Linden Require Import Regex Chars Groups.
 From Linden Require Import Tree Semantics NFA.
@@ -124,11 +125,11 @@ Definition add_thread_vt (seen:seenpcs) (t:thread_vt) : seenpcs :=
 
 (* the result of one step of exploring transitions *)
 Inductive epsilon_result_vt : Type :=
-| EpsActive: list thread_vt -> epsilon_result_vt
-| EpsMatch: epsilon_result_vt
-| EpsBlocked: thread_vt -> epsilon_result_vt.
+| EpsActive_vt: list thread_vt -> epsilon_result_vt
+| EpsMatch_vt: epsilon_result_vt
+| EpsBlocked_vt: thread_vt -> epsilon_result_vt.
 
-Definition EpsDead : epsilon_result_vt := EpsActive [].
+Definition EpsDead_vt : epsilon_result_vt := EpsActive_vt [].
 
 (* an atomic step for a thread *)
 (* TODO add regs as input and output: so that we can insert/split/delete *)
@@ -138,45 +139,45 @@ Definition epsilon_step_vt (t:thread_vt) (c:code) (i:input) (r:regs) : epsilon_r
       match get_pc c pc with
       | None =>
           let r' := Regs.delete ri r in
-          (EpsDead, r')
+          (EpsDead_vt, r')
       | Some instr =>
           match instr with
-          | Accept => (EpsMatch, r)
+          | Accept => (EpsMatch_vt, r)
           | Consume cd => match check_read rer cd i forward with
                           | CannotRead =>
                               let r' := Regs.delete ri r in
-                              (EpsDead, r')
-                          | CanRead => (EpsBlocked (block_thread_vt t), r)
+                              (EpsDead_vt, r')
+                          | CanRead => (EpsBlocked_vt (block_thread_vt t), r)
                          end
           | CheckAnchor a => match anchor_satisfied rer a i with
                              | false =>
                                  let r' := Regs.delete ri r in
-                                 (EpsDead, r')
-                             | true => (EpsActive [advance_thread_vt t], r)
+                                 (EpsDead_vt, r')
+                             | true => (EpsActive_vt [advance_thread_vt t], r)
                              end
-          | Jmp next => (EpsActive [upd_label_vt t next ri], r)
+          | Jmp next => (EpsActive_vt [upd_label_vt t next ri], r)
           | Fork l1 l2 =>
               let (r', ri') := (Regs.split ri r) in
-              (EpsActive [upd_label_vt t l1 ri; upd_label_vt t l2 ri'], r')
+              (EpsActive_vt [upd_label_vt t l1 ri; upd_label_vt t l2 ri'], r')
           | SetRegOpen gid =>
               let (t', r') := open_thread_vt t gid (idx i) r in
-              (EpsActive [t'], r')
+              (EpsActive_vt [t'], r')
           | SetRegClose gid =>
               let (t', r') := close_thread_vt t gid (idx i) r in
-              (EpsActive [t'], r')
+              (EpsActive_vt [t'], r')
           | ResetRegs gidl =>
               let (t', r') := reset_thread_vt t gidl r in
-              (EpsActive [t'], r')
-          | BeginLoop => (EpsActive [begin_thread_vt t], r)
+              (EpsActive_vt [t'], r')
+          | BeginLoop => (EpsActive_vt [begin_thread_vt t], r)
           | EndLoop next => match b with
                             | CannotExit =>
                                 let r' := Regs.delete ri r in
-                                (EpsDead, r')
-                            | CanExit => (EpsActive [upd_label_vt t next ri], r)
+                                (EpsDead_vt, r')
+                            | CanExit => (EpsActive_vt [upd_label_vt t next ri], r)
                             end
           | KillThread =>
               let r' := Regs.delete ri r in
-              (EpsDead, r')
+              (EpsDead_vt, r')
           end
       end
   end.
@@ -259,14 +260,14 @@ Inductive pike_vm_step_vt (c:code): pike_vm_state_vt -> pike_vm_state_vt -> Prop
   (* generated new active threads: add them in front of the low-priority ones *)
   forall inp t active best blocked nextprefix seen nextactive regs regs'
          (UNSEEN: seen_thread_vt seen t = false)
-         (STEP: epsilon_step_vt t c inp regs = (EpsActive nextactive, regs')), (* returns next regs *)
+         (STEP: epsilon_step_vt t c inp regs = (EpsActive_vt nextactive, regs')), (* returns next regs *)
     pike_vm_step_vt c (PVS_vt inp (t::active) best blocked nextprefix seen regs)
       (PVS_vt inp (nextactive++active) best blocked nextprefix (add_thread_vt seen t) regs')
 | pvs_match_vt:
   (* a match is found, discard remaining low-priority active threads *)
   forall inp t active best blocked nextprefix seen regs regs' regs''
          (UNSEEN: seen_thread_vt seen t = false)
-         (STEP: epsilon_step_vt t c inp regs = (EpsMatch, regs'))
+         (STEP: epsilon_step_vt t c inp regs = (EpsMatch_vt, regs'))
          (* delete regs of active threads (except t) and of previous best match *)
          (DELETE_REGS: regs'' = delete_thread_regs_from_regs_state active
                                   (delete_best_regs_from_regs_state best regs')),
@@ -276,7 +277,7 @@ Inductive pike_vm_step_vt (c:code): pike_vm_state_vt -> pike_vm_state_vt -> Prop
   (* add the new blocked thread after the previous ones *)
   forall inp t active best blocked nextprefix seen newt regs regs'
          (UNSEEN: seen_thread_vt seen t = false)
-         (STEP: epsilon_step_vt t c inp regs = (EpsBlocked newt, regs')), (* returns new regs *)
+         (STEP: epsilon_step_vt t c inp regs = (EpsBlocked_vt newt, regs')), (* returns new regs *)
     pike_vm_step_vt c (PVS_vt inp (t::active) best blocked nextprefix seen regs)
       (PVS_vt inp active best (blocked ++ [newt]) nextprefix (add_thread_vt seen t) regs').
 (* Unanchored PikeVM rules are removed: pvs_acc, pvs_nextchar_generate, pvs_next_char_filter *)
@@ -314,10 +315,185 @@ Definition leaves_equiv (res: option leaf) (res_vt: option leaf_vt) (r:regs) : P
   end.
 
 Definition thread_equiv (t: thread) (t_vt: thread_vt) (r: regs) : Prop :=
-  gm_vt_equiv (gm_of t) (ri_of t_vt) r.
+  match t, t_vt with
+    (l, gm, b), (l_vt, ri, b_vt) => l = l_vt /\ gm_vt_equiv gm ri r /\ b = b_vt
+  end.
 
 Definition threads_equiv (t: list thread) (t_vt: list thread_vt) (r: regs): Prop :=
   List.Forall2 (fun t t_vt => thread_equiv t t_vt r) t t_vt.
+
+Definition state_equiv (s: pike_vm_state) (s_vt: pike_vm_state_vt) : Prop :=
+  match s, s_vt with
+  | PVS i act best blo np seen, PVS_vt i' act' best' blo' np' seen' r =>
+      i = i' /\ np = np' /\ seen = seen' /\
+        threads_equiv act act' r /\ threads_equiv blo blo' r /\ leaves_equiv best best' r
+  | PVS_final best, PVS_final_vt best' r => leaves_equiv best best' r
+  | _, _ => False
+  end.
+
+Lemma seen_equiv : forall t t_vt seen r,
+    thread_equiv t t_vt r ->
+    seen_thread_vt seen t_vt = seen_thread seen t.
+Proof.
+  intros t t_vt seen r H.
+  unfold thread_equiv in *.
+  unfold seen_thread, seen_thread_vt in *.
+  destruct t as [[l gm] b].
+  destruct t_vt as [[l_vt ri] b_vt].
+  destruct H as [Hl [Hr Hb]].
+  subst.
+  reflexivity.
+Qed.
+
+Lemma epsilon_step_equiv_active :
+  forall c inp t t_vt nextactive_vt r r',
+    thread_equiv t t_vt r ->
+    epsilon_step_vt t_vt c inp r = (EpsActive_vt nextactive_vt, r') ->
+    (exists nextactive,
+        epsilon_step rer t c inp = EpsActive nextactive /\
+    threads_equiv nextactive nextactive_vt r').
+Admitted.
+
+Lemma epsilon_step_equiv_match :
+  forall c inp t t_vt r r',
+    thread_equiv t t_vt r ->
+    epsilon_step_vt t_vt c inp r = (EpsMatch_vt, r') ->
+    epsilon_step rer t c inp = EpsMatch /\ r = r'.
+Proof.
+  intros c inp t t_vt r r' Heq H.
+  unfold epsilon_step_vt, epsilon_step, thread_equiv in *.
+  destruct t_vt as [[l_vt ri] b_vt].
+  destruct t as [[l gm] b].
+  destruct Heq as [Hl [Hr Hb]]. subst.
+  destruct (get_pc c l_vt) eqn:BC.
+  - destruct b eqn:B;
+      try (injection H as H1 H2; inversion H1).
+    + injection H as H. subst.
+      auto.
+    + destruct (check_read rer c0 inp forward); injection H as H1 H2; inversion H1.
+    + destruct (anchor_satisfied rer a inp); injection H as H1 H2; inversion H1.
+    + destruct b_vt; injection H as H _; inversion H.
+  - injection H as H1 H2. inversion H1.
+Qed.
+
+Lemma epsilon_step_equiv_blocked :
+  forall c inp t t_vt newt_vt r r',
+    thread_equiv t t_vt r ->
+    epsilon_step_vt t_vt c inp r = (EpsBlocked_vt newt_vt, r') ->
+    (exists newt,
+        epsilon_step rer t c inp = EpsBlocked newt /\
+    thread_equiv newt newt_vt r').
+Admitted.
+
+Lemma pike_vm_step_vt_equiv :
+  forall c s s_vt s' s_vt',
+    (* s = (PVS inp act best blo None seen) *)
+    (* s_vt = (PVS inp act_vt best_vt blo_vt None seen regs) *)
+    state_equiv s s_vt ->
+    pike_vm_step rer c s s' ->
+    pike_vm_step_vt c s_vt s_vt' ->
+    state_equiv s' s_vt'.
+Proof.
+  unfold state_equiv.
+  intros c s s_vt s' s_vt' H STEP STEPVT.
+  dependent induction STEPVT; destruct s; try contradiction.
+  - (* pvs_final_vt *)
+    destruct H as [Hinp [Hnp [Hs [EQUIV_ACT [EQUIV_BLO EQUIV_LEA]]]]].
+    destruct active as [| t act]; inversion EQUIV_ACT; subst.
+    destruct blocked as [| t blo]; inversion EQUIV_BLO; subst.
+    inversion STEP. subst.
+    assumption.
+  - (* pvs_end_vt *)
+    destruct H as [Hinp [Hnp [Hs [EQUIV_ACT [EQUIV_BLO EQUIV_LEA]]]]].
+    destruct active as [| t act]; inversion EQUIV_ACT; subst.
+    destruct blocked0 as [| t blo]; inversion EQUIV_BLO; subst.
+    inversion STEP; subst; try congruence.
+    admit.
+  - (* pvs_nextchar_vt *)
+    destruct H as [Hinp [Hnp [Hs [EQUIV_ACT [EQUIV_BLO EQUIV_LEA]]]]].
+    inversion EQUIV_ACT. subst.
+    inversion EQUIV_BLO. subst.
+    inversion STEP; subst.
+    + congruence.
+    + repeat split; try assumption. congruence.
+  - (* pvs_skip_vt *)
+    destruct H as [Hinp [Hnp [Hs [EQUIV_ACT [EQUIV_BLO EQUIV_LEA]]]]].
+    destruct active0 as [| t act]; inversion EQUIV_ACT; subst.
+    apply seen_equiv with (seen:= seen) in H2; auto.
+    inversion STEP; subst; try (rewrite H2 in *; congruence).
+    admit.
+  - (* pvs_active_vt *)
+    destruct H as [Hinp [Hnp [Hs [EQUIV_ACT [EQUIV_BLO EQUIV_LEA]]]]].
+    destruct active0 as [| t act]; inversion EQUIV_ACT; subst.
+    specialize (epsilon_step_equiv_active _ _ _ _ _ _ _ H2 STEP0) as STEP1.
+    destruct STEP1 as [na [STEP1 Hna]].
+    apply seen_equiv with (seen:= seen) in H2; auto.
+    inversion STEP; subst; try (rewrite H12 in *; congruence); try congruence.
+    admit.
+  - (* pvs_match_vt *)
+    destruct H as [Hinp [Hnp [Hs [EQUIV_ACT [EQUIV_BLO EQUIV_LEA]]]]].
+    destruct active0 as [| t act]; inversion EQUIV_ACT; subst.
+    specialize (epsilon_step_equiv_match _ _ _ _ _ _ H2 STEP0) as [STEP1 Hr].
+    Print seen_equiv.
+    specialize (seen_equiv t t0 seen regs0 H2) as Hse.
+    inversion STEP; subst; try (rewrite H12 in *; congruence); try congruence.
+    repeat split; try reflexivity.
+    + admit.
+    + constructor.
+    + admit.
+    + unfold thread_equiv in *.
+      admit.
+  - (* pvs_blocked_vt *)
+    destruct H as [Hinp [Hnp [Hs [EQUIV_ACT [EQUIV_BLO EQUIV_LEA]]]]].
+    destruct active0 as [| t act]; inversion EQUIV_ACT; subst.
+    specialize (epsilon_step_equiv_blocked _ _ _ _ _ _ _ H2 STEP0) as STEP1.
+    destruct STEP1 as [nt [STEP1 Hnt]].
+    apply seen_equiv with (seen:= seen) in H2; auto.
+    inversion STEP; subst; try (rewrite H12 in *; congruence); try congruence.
+    admit.
+Admitted.
+
+Theorem trc_pikevm_vt_equiv: 
+  forall r s s_vt result result_vt regs,
+    state_equiv s s_vt ->
+    trc_pike_vm rer r s (PVS_final result) ->
+    trc_pike_vm_vt r s_vt (PVS_final_vt result_vt regs) ->
+    leaves_equiv result result_vt regs.
+Proof.
+  intros r s s_vt result result_vt regs EQUIV TRC TRCVT.
+  dependent induction TRC.
+  - unfold state_equiv in EQUIV.
+    destruct s_vt; try contradiction.
+    inversion TRCVT; subst.
+    + assumption.
+    + inversion STEP.
+  - inversion TRCVT. subst.
+    + unfold state_equiv in EQUIV.
+      destruct x; try contradiction.
+      inversion STEP.
+    + eapply IHTRC with (s_vt := y0).
+      * eapply pike_vm_step_vt_equiv; eauto.
+      * reflexivity.
+      * assumption.
+Qed.
+
+Theorem pikevm_vt_equiv: 
+  forall r inp result result_vt regs,
+  trc_pike_vm rer (compilation r) (pike_vm_initial_state inp) (PVS_final result) ->
+  trc_pike_vm_vt (compilation r) (pike_vm_initial_state_vt inp (regs_size_from_rer)) (PVS_final_vt result_vt regs) ->
+  leaves_equiv result result_vt regs.
+Proof.
+  intros r inp result result_vt regs TRC TRCVT.
+  eapply trc_pikevm_vt_equiv.
+  - admit.
+  - exact TRC.
+  - exact TRCVT.
+Admitted.
+
+
+
+
+(**************************)
 
 Lemma pike_vm_step_vt_equiv :
   forall c inp seen inp' seen'
@@ -325,9 +501,9 @@ Lemma pike_vm_step_vt_equiv :
          act' best' blo' act_vt' best_vt' blo_vt' regs',
     (* s = (PVS inp act best blo None seen) *)
     (* s_vt = (PVS inp act_vt best_vt blo_vt None seen regs) *)
-    threads_equiv act act_vt regs ->
-    threads_equiv blo blo_vt regs ->
-    leaves_equiv best best_vt regs ->
+    threads_equiv act act_vt regs /\
+      threads_equiv blo blo_vt regs /\
+      leaves_equiv best best_vt regs ->
     pike_vm_step rer c (PVS inp act best blo None seen)
       (PVS inp' act' best' blo' None seen') ->
     pike_vm_step_vt c (PVS_vt inp act_vt best_vt blo_vt None seen regs)
@@ -335,6 +511,46 @@ Lemma pike_vm_step_vt_equiv :
     threads_equiv act' act_vt' regs' /\
       threads_equiv blo' blo_vt' regs' /\
       leaves_equiv best' best_vt' regs'.
+Proof.
+  intros c inp seen inp' seen'
+         act best blo act_vt best_vt blo_vt regs
+         act' best' blo' act_vt' best_vt' blo_vt' regs'
+         [EQUIV_ACT [EQUIV_BLO EQUIV_BEST]] STEP STEP_VT.
+  dependent induction STEP_VT.
+  - (* pvs_nextchar_vt *)
+    inversion EQUIV_ACT. subst.
+    inversion STEP; subst.
+    repeat split; try assumption.
+  - (* pvs_skip_vt *)
+    destruct act as [| t act]; inversion EQUIV_ACT; subst.
+    apply seen_equiv with (seen:= seen') in H2; auto.
+    inversion STEP; subst; try (rewrite H12 in *; congruence).
+    admit.
+  - (* pvs_active_vt *)
+    destruct act as [| t act]; inversion EQUIV_ACT; subst.
+    specialize (epsilon_step_equiv_active _ _ _ _ _ _ _ H2 STEP0) as STEP1.
+    destruct STEP1 as [na [STEP1 Hna]].
+    apply seen_equiv with (seen:= seen) in H2; auto.
+    inversion STEP; subst; try (rewrite H12 in *; congruence); try congruence.
+    admit.
+  - (* pvs_match_vt *)
+    destruct act as [| t act]; inversion EQUIV_ACT; subst.
+    specialize (epsilon_step_equiv_match _ _ _ _ _ _ H2 STEP0) as [STEP1 Hr].
+    Print seen_equiv.
+    specialize (seen_equiv t t0 seen regs H2) as Hse.
+    inversion STEP; subst; try (rewrite H12 in *; congruence); try congruence.
+    repeat split.
+    + constructor.
+    + admit.
+    + unfold thread_equiv in *.
+      admit.
+  - (* pvs_blocked_vt *)
+    destruct act as [| t act]; inversion EQUIV_ACT; subst.
+    specialize (epsilon_step_equiv_blocked _ _ _ _ _ _ _ H2 STEP0) as STEP1.
+    destruct STEP1 as [nt [STEP1 Hnt]].
+    apply seen_equiv with (seen:= seen) in H2; auto.
+    inversion STEP; subst; try (rewrite H12 in *; congruence); try congruence.
+    admit.
 Admitted.
 
 Lemma pike_vm_step_vt_equiv_final :
@@ -343,9 +559,9 @@ Lemma pike_vm_step_vt_equiv_final :
          best' best_vt' regs',
     (* s = (PVS inp act best blo None seen) *)
     (* s_vt = (PVS inp act_vt best_vt blo_vt None seen regs) *)
-    threads_equiv act act_vt regs ->
-    threads_equiv blo blo_vt regs ->
-    leaves_equiv best best_vt regs ->
+    threads_equiv act act_vt regs /\
+      threads_equiv blo blo_vt regs /\
+      leaves_equiv best best_vt regs ->
     pike_vm_step rer c (PVS inp act best blo None seen)
       (PVS_final best') ->
     pike_vm_step_vt c (PVS_vt inp act_vt best_vt blo_vt None seen regs)
@@ -362,11 +578,153 @@ Admitted.
     pike_vm_state_equiv s' s_vt'.
 Admitted.*)
 
+Print trc.
+Lemma trc_consinv : forall (A: Type) (R: A -> A -> Prop) (x z: A),
+    @trc A R x z ->
+    x = z \/ (exists y, @trc A R x y /\ R y z).
+Proof.
+  intros A R x z H.
+  induction H.
+  - left. reflexivity.
+  - right.
+    destruct IHtrc as [Heq | [y' [Hxy Hyz]]].
+    + subst.
+      exists x.
+      split; [constructor | assumption].
+    + exists y'.
+      split.
+      * apply trc_cons with y; assumption.
+      * assumption.
+Qed.
+
+Lemma trc_tran : forall (A: Type) (R : A -> A -> Prop) (x y z: A),
+    @trc A R x y ->
+    @trc A R y z ->
+    @trc A R x z.
+Proof.
+  intros A R x y z Hxy Hyz.
+  induction Hxy.
+  - exact Hyz.
+  - apply trc_cons with (y := y).
+    + exact STEP.
+    + apply IHHxy.
+      exact Hyz.
+Qed.
+
+Lemma trc_pike_vm_vt_equiv_final :
+  forall c inp seen
+         act best blo act_vt best_vt blo_vt regs
+         best' best_vt' regs',
+    (* s = (PVS inp act best blo None seen) *)
+    (* s_vt = (PVS inp act_vt best_vt blo_vt None seen regs) *)
+    threads_equiv act act_vt regs /\
+      threads_equiv blo blo_vt regs /\
+      leaves_equiv best best_vt regs ->
+    trc_pike_vm rer c (PVS inp act best blo None seen)
+      (PVS_final best') ->
+    trc_pike_vm_vt c (PVS_vt inp act_vt best_vt blo_vt None seen regs)
+      (PVS_final_vt best_vt' regs') ->
+    leaves_equiv best' best_vt' regs'.
+Proof.
+  intros.
+  dependent induction H0.
+  eapply IHtrc.
+  - 
+  inversion H0; inversion H1; subst.
+Admitted.
+
+Print pike_vm_step.
+(*Lemma PVS_can_step :
+  forall c s s_vt res res_vt r',
+    pike_vm_step rer c s (PVS_final res) ->
+    pike_vm_step_vt c s_vt (PVS_final_vt res_vt r') ->
+    (exists inp act best blo np seen act_vt best_vt blo_vt np_vt seen_vt r,
+        s = PVS inp act best blo np seen /\
+          s_vt = PVS_vt inp act_vt best_vt blo_vt np_vt seen_vt r /\
+          leaves_equiv res res_vt r').
+Proof.
+  intros c s s_vt res res_vt r' H HVT.
+  inversion H; subst.
+  - repeat eexists.
+    inversion HVT; subst.
+    +  repeat eexists.
+  inversion HVT; subst; repeat eexists.
+  
+  inversion H; subst; repeat eexists.
+Qed.*)
+
+Lemma PVS_can_step :
+  forall c s s',
+    pike_vm_step rer c s s' ->
+    (exists inp act best blo np seen, s = PVS inp act best blo np seen).
+Proof.
+  intros c s s' H.
+  inversion H; subst; repeat eexists.
+Qed.
+
+Lemma PVS_can_step_vt :
+  forall c s s',
+    pike_vm_step_vt c s s' ->
+    (exists inp act best blo np seen r, s = PVS_vt inp act best blo np seen r).
+Proof.
+  intros c s s' H.
+  inversion H; subst; repeat eexists.
+Qed.
+
 Theorem pikevm_vt_equiv: 
   forall r inp result result_vt regs,
   trc_pike_vm rer (compilation r) (pike_vm_initial_state inp) (PVS_final result) ->
   trc_pike_vm_vt (compilation r) (pike_vm_initial_state_vt inp (regs_size_from_rer)) (PVS_final_vt result_vt regs) ->
   leaves_equiv result result_vt regs.
+Proof.
+  intros regex inp res res_vt r TRC TRC_VT.
+  dependent induction TRC_VT.
+  eapply IHTRC_VT in TRC_VT.
+  
+  unfold pike_vm_initial_state, pike_vm_initial_state_vt in *.
+  apply trc_consinv in TRC, TRC_VT.
+  destruct TRC as [TRC | [y [TRC TRC']]].
+  - inversion TRC.
+  - destruct TRC_VT as [TRC_VT | [y_vt [TRC_VT TRC_VT']]].
+    + inversion TRC_VT.
+    + specialize (PVS_can_step _ _ _ TRC')
+        as [i [act [best [blo [np [seen Hpvs]]]]]].
+      specialize (PVS_can_step_vt _ _ _ TRC_VT')
+        as [i' [act' [best' [blo' [np' [seen' [r' Hpvs']]]]]]].
+      subst.
+      eapply trc_pike_vm_vt_equiv_final. with
+        (inp:=inp) (c:=compilation regex) (seen:=initial_seenpcs)
+         (act:=[pike_vm_initial_thread]) (blo:=[]) (best:=None)
+         (act_vt:=[pike_vm_initial_thread_vt]) (blo_vt:=[]) (best_vt:=None) (regs:=r).
+  eapply trc_pike_vm_vt_equiv_final.
+  2: exact TRC.
+  2: exact TRC_VT.
+  split; try split.
+  - admit.
+  - constructor.
+  - simpl. tauto.
+  
+  unfold trc_pike_vm, trc_pike_vm_vt in *.
+  unfold pike_vm_initial_state, pike_vm_initial_state_vt in *.
+  inversion TRC; inversion TRC_VT; subst.
+  eapply pike_vm_step_vt_equiv_final.
+  2,3: econstructor
+  - admit.
+  - eapply pike_vm_step_vt_equiv.
+  1,2,3: admit.
+  - constructor.
+  - 
+  inversion TRC; inversion TRC_VT; subst.
+  unfold pike_vm_initial_state, pike_vm_initial_state_vt in *.
+  eapply pike_vm_step_vt_equiv_final
+    with (inp:=inp) (c:=compilation regex) (seen:=initial_seenpcs)
+         (act:=[pike_vm_initial_thread]) (blo:=[]) (best:=None)
+         (act_vt:=[pike_vm_initial_thread_vt]) (blo_vt:=[]) (best_vt:=None) (regs:=r).
+  - admit.
+  - constructor.
+  - simpl. tauto.
+  - admit.
+  
 Admitted.
 
 End PikeVM_VT.
